coq/src/Hacspec_Bls12_381.v
@@ -756,3 +756,40 @@ QuickChick (
   forAll g_fp12_t (fun a_325 : fp12_t =>test_fp12_prop_mul_inv a_325)).
 
 
+Definition scalar_canvas_t := nseq (int8) (32).
+Definition scalar_t :=
+  nat_mod 0x8000000000000000000000000000000000000000000000000000000000000000.
+
+Notation "'g1_t'" := ((fp_t × fp_t × bool)) : hacspec_scope.
+
+Notation "'fp2_t'" := ((fp_t × fp_t)) : hacspec_scope.
+
+Notation "'g2_t'" := ((fp2_t × fp2_t × bool)) : hacspec_scope.
+
+Notation "'fp6_t'" := ((fp2_t × fp2_t × fp2_t)) : hacspec_scope.
+
+Notation "'fp12_t'" := ((fp6_t × fp6_t)) : hacspec_scope.
+
+Definition fp_return_zero  : fp_t :=
+  nat_mod_zero .
+
+Theorem ensures_fp_return_zero : forall result_0 ,
+ @fp_return_zero  = result_0 ->
+ ((nat_mod_model (result_0)) =.? (usize 0)) = true.
+Proof.
+  intros.
+  subst.
+  reflexivity.
+Qed.
+
+Definition fp2fromfp (n_1 : fp_t) : fp2_t :=
+  (n_1, nat_mod_zero ).
+
+Definition fp2zero  : fp2_t :=
+  fp2fromfp (nat_mod_zero ).
+
+Definition fp2neg (n_2 : fp2_t) : fp2_t :=
+  let '(n1_3, n2_4) :=
+    n_2 in 
+  ((nat_mod_zero ) -% (n1_3), (nat_mod_zero ) -% (n2_4)).
+
